

Power series method

Example ①: Solve $y'' = y$

We assume that the solution $y(x)$ can be written as a power series in x , i.e.,

$$\begin{aligned} y(x) &= a_0 + a_1 x + a_2 x^2 + \dots + a_n x^n + \dots \\ &= \sum_{n=0}^{\infty} a_n x^n \end{aligned}$$

Then by the term-by-term differentiation,

$$y'(x) = \sum_{n=1}^{\infty} n a_n x^{n-1}$$

$$\& \quad y''(x) = \sum_{n=2}^{\infty} n(n-1) a_n x^{n-2}$$

$y(x)$ is a soln. to $y'' = y$ iff

$$\underbrace{\sum_{n=2}^{\infty} n(n-1)a_n x^{n-2}}_{=} = \sum_{n=0}^{\infty} a_n x^n$$

$$\sum_{n=0}^{\infty} (n+2)(n+1)a_{n+2} x^n$$

$$\Rightarrow \sum_{n=0}^{\infty} [(n+2)(n+1)a_{n+2} - a_n] x^n = 0$$

$$\Rightarrow (n+2)(n+1)a_{n+2} - a_n = 0$$

$$\Rightarrow \boxed{a_{n+2} = \frac{a_n}{(n+2)(n+1)} \text{ for all } n=0,1,2,\dots}$$

→ recurrence relation.

$$\text{Put } n=0 : a_2 = \frac{a_0}{2 \times 1} = \frac{a_0}{2!}$$

$$\text{Put } n=2 : a_4 = \frac{a_2}{4 \times 3} = \frac{a_0}{4 \times 3 \times 2 \times 1} = \frac{a_0}{4!}$$

$$\text{Inductively, } \boxed{a_{2n} = \frac{a_0}{(2n)!}} \text{ for } n=0,1,2,\dots$$

Putting $n=1$, we get

$$a_3 = \frac{a_1}{3 \times 2} = \frac{a_1}{3!}$$

Put $n=3$: $a_5 = \frac{a_3}{5 \times 4} = \frac{a_1}{5!}$

$$\therefore \boxed{a_{2n+1} = \frac{a_1}{(2n+1)!} \text{ for } n=1,2,3,\dots}$$

$$\begin{aligned} \therefore y &= \sum_{n=0}^{\infty} a_n x^n \\ &= \sum_{n=0}^{\infty} a_{2n} x^{2n} + \sum_{n=0}^{\infty} a_{2n+1} x^{2n+1} \\ &= \sum_{n=0}^{\infty} \frac{a_0}{(2n)!} x^{2n} + \sum_{n=0}^{\infty} \frac{a_1}{(2n+1)!} x^{2n+1} \\ &= a_0 \sum_{n=0}^{\infty} \frac{x^{2n}}{(2n)!} + a_1 \sum_{n=0}^{\infty} \frac{x^{2n+1}}{(2n+1)!} \\ &= a_0 y_1(x) + a_1 y_2(x) \end{aligned}$$

Note that

$$\begin{aligned}y_1(x) &= \sum_{n=0}^{\infty} \frac{x^{2n}}{(2n)!} \\&= 1 + \frac{x^2}{2!} + \frac{x^4}{4!} + \frac{x^6}{6!} + \dots \\&= \frac{e^x + e^{-x}}{2}\end{aligned}$$

$$\begin{aligned}\text{and } y_2(x) &= \sum_{n=0}^{\infty} \frac{x^{2n+1}}{(2n+1)!} \\&= \frac{e^x - e^{-x}}{2}\end{aligned}$$

$$\begin{aligned}\therefore y(x) &= a_0 \left(\frac{e^x + e^{-x}}{2} \right) + a_1 \left(\frac{e^x - e^{-x}}{2} \right) \\&= c_1 e^x + c_2 e^{-x}, \\&\text{where } c_1 = \frac{a_0 + a_1}{2} \\&\quad c_2 = \frac{a_0 - a_1}{2}.\end{aligned}$$

Example (2) Solve $y'' + y = 0$
by using power series method.

Let $y = \sum_{n=0}^{\infty} a_n x^n$

Then $y' = \sum_{n=1}^{\infty} n a_n x^{n-1}$

$$y'' = \sum_{n=2}^{\infty} n(n-1) a_n x^{n-2}$$

$$= \sum_{n=0}^{\infty} (n+2)(n+1) a_{n+2} x^n$$

$$\therefore \sum_{n=0}^{\infty} [(n+2)(n+1) a_{n+2} + a_n] x^n = 0$$

$$\Rightarrow a_{n+2} = \frac{-a_n}{(n+2)(n+1)} \text{ for } n=0,1,2,\dots$$

$$\Rightarrow a_{2n} = \frac{(-1)^n a_0}{(2n)!} \text{ for } n=0,1,2,\dots$$

$$a_{2n+1} = \frac{(-1)^n a_1}{(2n+1)!} \text{ for } n=0,1,2,\dots$$

$$\begin{aligned}
 \therefore y &= \sum_{n=0}^{\infty} a_{2n} x^{2n} + \sum_{n=0}^{\infty} a_{2n+1} x^{2n+1} \\
 &= \sum_{n=0}^{\infty} \frac{(-1)^n a_0 x^{2n}}{(2n)!} + \sum_{n=0}^{\infty} \frac{(-1)^n a_1 x^{2n+1}}{(2n+1)!} \\
 &= a_0 \underbrace{\sum_{n=0}^{\infty} \frac{(-1)^n x^{2n}}{(2n)!}}_{\substack{\text{||} \\ 1 - \frac{x^2}{2!} + \frac{x^4}{4!} - \dots \\ \text{||} \\ \cos x}} + a_1 \underbrace{\sum_{n=0}^{\infty} \frac{(-1)^n x^{2n+1}}{(2n+1)!}}_{\substack{\text{||} \\ \sin x}}
 \end{aligned}$$

$$\therefore y = a_0 \cos x + a_1 \sin x$$

When is the power series applicable?

Theorem: Consider the linear ODE of the form $y'' + p(x)y' + q(x)y = r(x)$.

Suppose $p(x)$, $q(x)$ and $r(x)$ can be expressed as power series in x (or about $x=a$). Then the solution $y(x)$ can be written

as a power series $\sum_{n=0}^{\infty} a_n x^n$ (or $\sum_{n=0}^{\infty} a_n (x-a)^n$)

Remark. (i) The above theorem is valid for any n th order linear ODE also.

(ii) Generally, we use this method when $p(x)$, $q(x)$, $r(x)$ are polynomials.

Example (3): Solve $y'' + xy = 0$.

$$\text{Let } y = \sum_{n=0}^{\infty} a_n x^n$$

$$\Rightarrow y'' = \sum_{n=0}^{\infty} (n+2)(n+1) a_{n+2} x^n$$

$$\therefore \sum_{n=0}^{\infty} (n+2)(n+1) a_{n+2} x^n + x \sum_{n=0}^{\infty} a_n x^n = 0$$

$$\Rightarrow \sum_{n=0}^{\infty} (n+2)(n+1) a_{n+2} x^n + \sum_{n=0}^{\infty} a_n x^{n+1} = 0$$

$$\text{Coeff. of } x^0: 2a_2 = 0 \Rightarrow \boxed{a_2 = 0}$$

$$\text{Coeff. of } x^{n+1} (n \geq 0): (n+3)(n+2) a_{n+3} + a_n = 0$$

$$\Rightarrow \boxed{a_{n+3} = \frac{-a_n}{(n+3)(n+2)}} \text{ for } n=0, 1, 2, \dots$$

Since $a_2 = 0$, we get $a_5 = 0 = a_8 = a_{11} = \dots$

$$\therefore \boxed{a_{2+3k} = 0 \text{ for } k=0, 1, 2, \dots}$$

Putting $n=0$: $a_3 = \frac{-a_0}{3 \times 2} = -\frac{a_0}{6}$

Put $n=3$: $a_6 = \frac{-a_3}{6 \times 5} = \frac{a_0}{30 \times 6} = \frac{a_0}{180}$,

Put $n=6$: $a_9 = \frac{-a_6}{9 \times 8 \times 180}$, ...

Put $n=1$: $a_4 = \frac{-a_1}{12}$

$n=4$: $a_7 = \frac{-a_4}{7 \times 6} = \frac{a_1}{42 \times 12}$

We can find as many terms as we want.

$$y = a_0 \left[1 - \frac{1}{6}x^3 + \frac{1}{180}x^6 - + \dots \right] \\ + a_1 \left[x - \frac{1}{12}x^4 + \frac{1}{504}x^7 - + \dots \right]$$

Exercise: Solve the following using the power series method:

① $y'' - xy' + y = 0$

② $y'' - y' = 0$

③ $(2x^2 - 3x + 1)y'' + 2xy' - 2y = 0$

Remark: For ①, note that $y = x$ is a solution. Try to find a second linearly indep. soln. using the reduction of order method.

Ref: Chapter 5.1 in Kreyszig.